Veritas.SeqAux.fst
@@ -203,6 +203,20 @@ let lemma_not_exists_prefix (#a:eqtype) (f:a -> bool) (s:seq a) (i:nat{i <= leng
   )
   else ()
 
+let lemma_last_index_last_elem_nsat (#a:eqtype) (f:a -> bool) (s:seq a{length s > 0}):
+  Lemma (requires (not (f (index s (length s - 1)))))
+        (ensures (exists_sat_elems f s ==> last_index f s < length s - 1)) = 
+  if exists_sat_elems f s then
+    let li = last_index f s in
+    ()
+  else ()
+
+let lemma_last_index_last_elem_sat (#a:eqtype) (f:a -> bool) (s:seq a{length s > 0}):
+  Lemma (requires (f (index s (length s - 1))))
+        (ensures (exists_sat_elems f s /\ last_index f s = length s - 1)) =
+  let n = length s in
+  lemma_last_index_correct2 f s (n - 1)
+
 let first_index (#a:eqtype) (f:a -> bool) (s:seq a{exists_sat_elems f s})
   : Tot (i:seq_index s{f (index s i)}) =
   filter_index_inv_map f s 0
